pcuic/theories/PCUICWeakening.v
@@ -154,9 +154,7 @@ Lemma lift_unfold_fix n k mfix idx narg fn :
 Proof.
   unfold unfold_fix.
   rewrite nth_error_map. destruct (nth_error mfix idx) eqn:Hdef; try congruence.
-  case e: isLambda => //.
   intros [= <- <-]. simpl.
-  rewrite isLambda_lift //.
   repeat f_equal.
   rewrite (distr_lift_subst_rec _ _ n 0 k).
   rewrite fix_subst_length. f_equal.
